lib/DataStructures/KMBtree.i.dfy
@@ -1,4 +1,5 @@
 include "MutableBtreeBulkOperations.i.dfy"
+include "MutableBtree.i.dfy"
 include "../Base/Message.i.dfy"
   
 module KMBtreeModel refines BtreeModel {
@@ -7,7 +8,7 @@ module KMBtreeModel refines BtreeModel {
   type Value = Messages.Message
 }
 
-module KMBtree refines MutableBtree {
+module LKMBtree refines LMutableBtree {
   import Model = KMBtreeModel
     
   function method MaxKeysPerLeaf() : uint64 { 64 }
@@ -17,6 +18,12 @@ module KMBtree refines MutableBtree {
   function method DefaultKey() : Key { [] }
 }
 
+module KMBtree refines MutableBtree {
+  import L = LKMBtree`All
+  import Model = KMBtreeModel
+}
+
+// TODO(robj): dead code; delete?
 module KMBtreeBulkOperations refines MutableBtreeBulkOperations {
   import opened MB = KMBtree`All
 }
